disk-betree/ImplModelIO.i.dfy
@@ -124,7 +124,7 @@ module ImplModelIO {
     Marshalling.reveal_parseSector();
   }
 
-  predicate FindLocationAndRequestWrite(io: IO, s: Variables, sector: Sector, id: Option<D.ReqId>, loc: Option<LBAType.Location>, io': IO)
+  predicate {:opaque} FindLocationAndRequestWrite(io: IO, s: Variables, sector: Sector, id: Option<D.ReqId>, loc: Option<LBAType.Location>, io': IO)
   requires s.Ready?
   requires WFVars(s)
   {
